

1.

1) FSPA, $r \geq 0$, $n \geq 2$. Winner pays second-highest if exists, o.w, own.

$$m(x) = \int_{v_0}^{v_0} \beta(x) dG(z) + \int_{v_0}^x \beta(z) dG(z) + \int_x^{\bar{v}} 0 dG(z)$$

i wins, no other i wins, others i loses

$$= \beta(x) G(v_0) + \int_{v_0}^x \beta(z) dG(z)$$

BC: marginal type v_0 , assume $m(x)$ increasing in $\beta(x)$

$\beta(v_0) = r$ lowest possible bid.

$$m(v_0) = \beta(v_0) G(v_0) + \int_{v_0}^{v_0} \beta(z) dG(z)$$

"0

$$\stackrel{*}{=} r G(v_0)$$

$$IC: U(v, v_0) = v_0 G(v_0) - m(v_0) = 0$$

$$\Rightarrow v_0 G(v_0) - r G(v_0) = 0$$

$$\Rightarrow (v_0 - r) G(v_0) = 0$$

so, $v_0 = r$, same as in FPA, $r \geq 0$

$$U(x; v) = v G(x) - m(x)$$

$$= v G(x) - (\beta(x) G(v_0) + \int_{v_0}^x \beta(z) dG(z))$$

done above

2) 3) 4) 5)

LEIBNIZ RULE:

$$\frac{d}{dx} \int_{a(x)}^{b(x)} f(x, t) dt$$

$$= f(x, b(x)) b'(x) -$$

$$f(x, a(x)) a'(x) +$$

$$\int_{a(x)}^{b(x)} \frac{d}{dx} f(x, t) dt$$

"Leibniz: $\beta(x) G'(x)$

$$RP: U'(x; v) = v G' - \beta' G(v_0) - \frac{d}{dx} \int_{v_0}^x \beta(z) dG(z)$$

$$= v G' - \beta' G(v_0) - \beta(x) G'(x)$$

Letting $U'(x, x) = 0$, $n=2$, $F(x) = x$, $G(x) = x$, $G'(x) = 1$

$$\text{gives : } \beta'(x) = -\frac{1}{v_0} \beta(x) + \frac{1}{v_0} v \quad (2)$$

By appendix A.3, $y'(x) = a(x)y(x) + b(x)$ giving:

$$\begin{aligned} y(x) &= \exp \left\{ \int_{x_0}^x a(t) dt \right\} \left(y(x_0) + \int_{x_0}^x b(z) \exp \left\{ - \int_{x_0}^z a(t) dt \right\} dz \right) \\ &= \exp \left\{ \int_{v_0}^x -\frac{1}{v_0} dt \right\} \left(\beta(v_0) + \int_{v_0}^x \frac{1}{v_0} y \exp \left\{ - \int_{v_0}^y -\frac{1}{v_0} dt \right\} dy \right) \\ &\stackrel{BC}{=} \exp \left\{ -\frac{1}{v_0}(x-v_0) \right\} \left(r + \int_{v_0}^x \frac{1}{v_0} y \exp \left\{ \frac{1}{v_0}(y-v_0) \right\} dy \right) \\ &= \exp \left\{ 1 - \frac{x}{v_0} \right\} \left(r + \int_{v_0}^x \frac{1}{v_0} (y \exp \left\{ \frac{y}{v_0} - 1 \right\}) dy \right) \end{aligned}$$

$$\begin{aligned} * \int_{v_0}^x y \exp \left\{ \frac{y}{v_0} - 1 \right\} dy &= \frac{1}{e} \int_{v_0}^x y e^{y/v_0} dy \\ &= \frac{1}{e} \left([v_0 y e^{y/v_0}]_{v_0}^x - \int_{v_0}^x (v_0 e^{y/v_0}) dy \right) \\ &= \frac{1}{e} v_0 \left(x e^{x/v_0} - v_0 e - [v_0 e^{y/v_0}]_{v_0}^x \right) \\ &= \frac{1}{e} v_0 \left(x e^{x/v_0} - v_0 e - v_0 e^{x/v_0} + v_0 e \right) \\ &= v_0 x e^{\frac{x}{v_0}-1} - v_0^2 e^{\frac{x}{v_0}-1} \\ &= v_0 e^{\frac{x}{v_0}-1} (x - v_0) \end{aligned}$$

$$\begin{aligned} * &= e^{1-\frac{x}{v_0}} \left(r + e^{\frac{x}{v_0}-1} (x - v_0) \right) \\ &= r e^{1-\frac{x}{v_0}} + x - v_0 \end{aligned}$$

$$\begin{aligned} \text{Hence } \beta(v, v_0, r) &= v - v_0 + r e^{1-\frac{v}{v_0}} \\ \beta(v, r) &= v - r + r e^{1-\frac{v}{r}} \quad w/ v \geq r \quad (3) \end{aligned}$$

$$\begin{aligned} m(x) &= \beta(x) G(v_0) + \int_{v_0}^x \beta(z) dG(z) \\ &= xr - r^2 + r^2 e^{1-\frac{x}{r}} + \int_r^x (z - r + r e^{1-\frac{z}{r}}) dz \\ &= xr - r^2 + r^2 e^{1-\frac{x}{r}} + \left[\frac{1}{2} z^2 - rz \right]_r^x - \left[r^2 e^{1-\frac{z}{r}} \right]_r^x \\ &= xr - r^2 + r^2 e^{1-\frac{x}{r}} + \frac{1}{2} x^2 - rx + \frac{1}{2} r^2 + r^2 (1 - e^{1-\frac{x}{r}}) \\ &= \frac{1}{2} (x^2 + r^2) \end{aligned}$$

Prop. 3.1 says

PROPOSITION 3.1 (The Expected Payment Result). In an MSPE of any standard auctions with marginal type v_0 , a bidder of type $v \in [v_0, \bar{v}]$ in expectation pays:

$$m(v) = v_0 G(v_0) + \int_{v_0}^v x dG(x) = vG(v) - \int_{v_0}^v G(x) dx.$$

$$\begin{aligned} m(v) &= v_0^2 + \int_{v_0}^v x dx \\ &= v_0^2 + \frac{1}{2} [x^2]_{v_0}^v \\ &= \frac{1}{2} v^2 + \frac{1}{2} v_0^2 \end{aligned}$$

since in our question $v_0 = r$, $m(v)$ equivalent
as above ⑤

